\subsubsection{The beta distribution}
\begin{definition}
Gamma function is defined as $\gamma(x)=\int_{0}^{\infty}t^{x-1}e^{-t}\text{d}t$\\
which converges for $x>0$.
\end{definition}
\begin{conclusion}
$\gamma$ function is the generalization of factorial for real and complex numbers.
\begin{equation}
\gamma(x+1)=x\gamma(x)
\label{eqn:factorialgamma}
\end{equation}
\end{conclusion}
\begin{proof}
(Integration by parts) 
\begin{equation}
\begin{split}
\gamma(x+1)&=\int_{0}^{\infty}t^{x}e^{-t}\text{d}t\\
&=-\int_{0}^{\infty}t^{x}\frac{\text{d}e^{-t}}{\text{d}t}\text{d}t\\
&=-t^{x}e^{-t}\vert_{0}^{\infty}+\int_{0}^{\infty}xt^{x-1}e^{-t}\text{d}t\\
&=x\gamma(x)
\end{split}
\end{equation}
\end{proof}
The conjugate prior is \emph{beta} distribution:
\begin{definition}
\begin{equation}
\text{Beta}(\mu\vert{}a,b)=\frac{\Gamma(a+b)}{\Gamma(a)\Gamma(b)}\mu^{a-1}(1-\mu)^{b-1}
\label{eqn:betadist}
\end{equation}
which is well defined when $a,b\geq{}0$.
\end{definition}
(Ex 2.5) Beta distribution is normalized:
\begin{proof}
It is equivalent to prove $\int_{0}^{1}\mu^{a-1}(1-\mu)^{b-1}\text{d}\mu=\frac{\Gamma(a)\Gamma(b)}{\Gamma(a+b)}$.


According to definition of gamma function, $\Gamma(a)\Gamma(b)=\int_{0}^{\infty}\exp{}(-x)x^{a-1}\text{d}x\int_{0}^{\infty}\exp{}(-y)y^{b-1}\text{d}y$.



Firstly, substitute $y$ by $t$ where $t=y+x$ resulting $\int_{0}^{\infty}\int_{0}^{\infty}\exp{}(-t)x^{a-1}(t-x)^{b-1}\text{d}t\text{d}x$


Secondly, substitute $x$ by $\mu$ where $x=t\mu$. $\because\text{d}x=t\text{d}\mu$
\begin{equation}
\begin{split}
\therefore\Gamma(a)\Gamma(b)&=\int_{0}^{1}\int_{0}^{\infty}\exp{}(-t)(t\mu)^{a-1}(t-t\mu)^{b-1}t\text{d}t\text{d}\mu\\
&=\int_{0}^{1}\{\int_{0}^{\infty}\exp{}(-t)t^{a+b-1}\text{d}t\}\mu^{a-1}(1-\mu)^{b-1}\text{d}\mu\\
&=\Gamma(a+b)\int_{0}^{1}\mu^{a-1}(1-\mu)^{b-1}\text{d}\mu
\end{split}
\label{eqn:gammaasintcircle}
\end{equation}
\end{proof}
\begin{conclusion}
(Ex 2.6) The mean of beta distribution is given by $\mathbb{E}[\mu]=\frac{a}{a+b}$
\end{conclusion}
\begin{proof}
\begin{equation}
\begin{split}
\int_{0}^{1}\mu\text{Beta}(\mu)\text{d}\mu&=\frac{\Gamma(a+b)}{\Gamma(a)\Gamma(b)}\int_{0}^{1}\mu^{(a+1)-1}(1-\mu)^{b-1}\text{d}\mu\\
&=\frac{\Gamma(a+b)}{\Gamma(a)\Gamma(b)}\frac{\Gamma(a+1)\Gamma(b)}{\Gamma(a+b+1)}\quad(\because\text{\eqref{eqn:gammaasintcircle}})\\
&=\frac{\Gamma(a+1)}{\Gamma(a)}\frac{\Gamma(a+b)}{\Gamma(a+b+1)}=\frac{a}{a+b}\\
\end{split}
\end{equation}
\end{proof}
In a similar way, we can prove that $\text{var}[\mu]=\frac{ab}{(a+b)^2(a+b+1)}$.
